examples/iterators/FindMax.dfy
@@ -4,31 +4,29 @@ include "../../src/linear/layer2/ArrayList.dfy"
 
 method FindMax(l: LinkedList<int>) returns (max: ListIterator<int>)
   modifies l, l.Repr()
+  requires allocated(l.Repr())
+
   requires l.Valid()
   requires l.Model() != []
-  requires forall x | x in l.Repr() :: allocated(x)
-  
   ensures l.Valid()
   ensures l.Model() == old(l.Model())
   ensures fresh(max) && max in l.Iterators()
   ensures max.Valid()
   ensures max.Parent() == l
-  ensures max.HasNextF()
+  ensures max.HasNext?()
   ensures forall x | x in l.Model() :: l.Model()[max.Index()] >= x
+
+  ensures fresh(l.Repr()-old(l.Repr()))
+  ensures allocated(l.Repr())
 
   ensures l.Iterators() >= old(l.Iterators())
   ensures forall it | it in old(l.Iterators()) && old(it.Valid()) ::
-    it.Valid() && it.Index() == old(it.Index())
-
-  ensures forall x {:trigger x in l.Repr(), x in old(l.Repr())} | x in l.Repr() - old(l.Repr()) :: fresh(x)
-  ensures forall x | x in l.Repr() - old(l.Repr()) :: fresh(x)
-  ensures forall x | x in l.Repr() :: allocated(x)
+    it.Valid() && it.Parent()==old(it.Parent()) && it.Index() == old(it.Index())
 
 {
   max := l.Begin();
   var it := l.Begin();
   var b:=it.HasNext(); //Nuevo
-  var itPeek, maxPeek;
 
   while b
     decreases |l.Model()| - it.Index()
@@ -41,24 +39,25 @@ method FindMax(l: LinkedList<int>) returns (max: ListIterator<int>)
     invariant max.Parent() == l
     invariant max in l.Iterators()
     invariant max != it
-    invariant max.HasNextF()
+    invariant max.HasNext?()
     invariant it.Index() <= |l.Model()|
     invariant forall k | 0 <= k < it.Index() :: l.Model()[max.Index()] >= l.Model()[k]
-    invariant b == it.HasNextF()
+    invariant b == it.HasNext?()
+
+    invariant allocated(l.Repr())
+    invariant fresh(l.Repr()-old(l.Repr()))
 
     invariant l.Iterators() >= old(l.Iterators())
     invariant forall it | it in old(l.Iterators()) && old(it.Valid()) ::
-      it.Valid() && it.Index() == old(it.Index())
+      it.Valid() && it.Parent()==old(it.Parent()) && it.Index() == old(it.Index())
 
-    invariant forall x {:trigger x in l.Repr(), x in old(l.Repr())} | x in l.Repr() && x !in old(l.Repr()) :: fresh(x)
-    invariant forall x | x in l.Repr() :: allocated(x)
-    invariant forall x | x in old(l.Repr()) :: allocated(x)  
-  { itPeek:= it.Peek(); maxPeek:= max.Peek();
+  { var itPeek:= it.Peek(); 
+    var maxPeek:= max.Peek();
 
     if itPeek > maxPeek {
       max := it.Copy();
     }
-    var x := it.Next();
+    var _ := it.Next();
     b:=it.HasNext();
   }
 }
@@ -66,29 +65,29 @@ method FindMax(l: LinkedList<int>) returns (max: ListIterator<int>)
 
 method FindMaxAL(l: ArrayList<int>) returns (max: ListIterator<int>)
   modifies l, l.Repr()
+  requires allocated(l.Repr())
+
   requires l.Valid()
   requires l.Model() != []
-  requires forall x | x in l.Repr() :: allocated(x)
   ensures l.Valid()
   ensures l.Model() == old(l.Model())
   ensures fresh(max) && max in l.Iterators()
   ensures max.Valid()
   ensures max.Parent() == l
-  ensures max.HasNextF()
+  ensures max.HasNext?()
   ensures forall x | x in l.Model() :: l.Model()[max.Index()] >= x
+
+  ensures fresh(l.Repr()-old(l.Repr()))
+  ensures allocated(l.Repr())
 
   ensures l.Iterators() >= old(l.Iterators())
   ensures forall it | it in old(l.Iterators()) && old(it.Valid()) ::
-    it.Valid() && it.Index() == old(it.Index())
+    it.Valid() && it.Parent()==old(it.Parent()) && it.Index() == old(it.Index())
 
-  ensures forall x {:trigger x in l.Repr(), x in old(l.Repr())} | x in l.Repr() - old(l.Repr()) :: fresh(x)
-  ensures forall x | x in l.Repr() - old(l.Repr()) :: fresh(x)
-  ensures forall x | x in l.Repr() :: allocated(x)  
 {
   max := l.Begin();
   var it := l.Begin();
-  var b:=it.HasNext(); //Nuevo
-  var itPeek, maxPeek;
+  var b:=it.HasNext();
 
   while b
     decreases |l.Model()| - it.Index()
@@ -102,26 +101,27 @@ method FindMaxAL(l: ArrayList<int>) returns (max: ListIterator<int>)
     invariant max.Parent() == l
     invariant max in l.Iterators()
     invariant max != it
-    invariant max.HasNextF()
+    invariant max.HasNext?()
     invariant it.Index() <= |l.Model()|
     invariant forall k | 0 <= k < it.Index() :: l.Model()[max.Index()] >= l.Model()[k]
-    invariant b == it.HasNextF()
+    invariant b == it.HasNext?()
     
+    invariant allocated(l.Repr())
+    invariant fresh(l.Repr()-old(l.Repr()))
+
     invariant l.Iterators() >= old(l.Iterators())
     invariant forall it | it in old(l.Iterators()) && old(it.Valid()) ::
       it.Valid() && it.Index() == old(it.Index())
-
-    invariant forall x {:trigger x in l.Repr(), x in old(l.Repr())} | x in l.Repr() && x !in old(l.Repr()) :: fresh(x)
-    invariant forall x | x in l.Repr() :: allocated(x)
-    invariant forall x | x in old(l.Repr()) :: allocated(x)  
   {
-    itPeek:= it.Peek(); maxPeek:= max.Peek();
+    var itPeek:= it.Peek(); 
+    var maxPeek:= max.Peek();
 
     if itPeek > maxPeek {
       max := it.Copy();
     }
-    var x := it.Next();
+    var _ := it.Next();
     
     b:=it.HasNext();
   }
 }
+
